promising check point

monad/smonad2.v
@@ -1,5 +1,6 @@
 Require Import Program.
 
+Section monad.
 Variable ST : Set.
 
 Definition ST_Pre : Type
@@ -7,23 +8,22 @@ Definition ST_Pre : Type
 Definition ST_Post (A:Set) : Type :=
   ST -> A -> ST -> Prop.
 Definition C_Post (A:Set) : Type :=
-  A -> nat -> Prop.
+  ST -> A -> nat -> ST -> Prop.
 
 Program Definition
   CS (st_pre : ST_Pre) (A : Set) (st_post : ST_Post A)
      (c_post : C_Post A) : Set :=
   forall st : { st : ST | st_pre st },
     { (a, st') : A * ST | st_post st a st' /\
-      (* xxx what if the proof requires knowing st_post? 
-             what if the proof needs to mention the store? *)
-      exists an, c_post a an }.
+      (* xxx what if the proof requires knowing st_post? *)
+      exists an, c_post st a an st' }.
 Hint Unfold CS.
 
 Definition top : ST_Pre := fun st => True.
 
 Program Definition ret (A : Set) (c_post : C_Post A) 
   : forall av,
-    c_post av 0 ->
+    (forall st, c_post st av 0 st) ->
     CS top A (fun st ap st' => st = st' /\ ap = av) c_post.
 Proof.
   intros A c_post av CPav0.
@@ -31,7 +31,7 @@ Proof.
   intros [st st_pre_st].
   exists (av, st).
   eauto.
-Qed.
+Defined.
 
 Program Definition bind:
   forall (A B:Set)
@@ -41,10 +41,10 @@ Program Definition bind:
     (CS st_preA A st_postA c_postA) ->
     (forall (a : A), (* xxx missing (pa:exists an, PA a an) from monad.v *)
       (CS (st_preB a) B (st_postB a)
-        (fun b bn =>
-          forall an,
-            c_postA a an ->
-            c_postB b (an+bn)))) ->
+        (fun stA b bn stB =>
+          forall st0 an,
+            c_postA st0 a an stA ->
+            c_postB st0 b (an+bn) stB))) ->
     CS (fun st0 =>
       st_preA st0 /\
       (forall a stA,
@@ -72,35 +72,34 @@ Proof.
 
   destruct c_postA_stA as [an c_postA_stA].
   destruct c_postApostB_stB as [bn c_postApostB_stB].
-  exists (an + bn).
-  eauto.
-Qed.
+  exists (an + bn). eauto.
+Defined.
 
 Program Definition get:
   CS top ST (fun st0 st1 st2 => st0 = st1 /\ st1 = st2)
-  (fun st1 st1n => st1n = 0).
+  (fun _ st1 st1n _ => st1n = 0).
 Proof.
   intros [st0 st_pre_st0].
   exists (st0, st0). simpl.
   eauto.
-Qed.
+Defined.
 
 Program Definition put (st2:ST) :
   CS top () (fun _ _ st2' => st2 = st2')
-  (fun _ un => un = 0).
+  (fun _ _ un _ => un = 0).
 Proof.
   intros st2 [st0 st_pre_st0].
   exists ((), st2).
   eauto.
-Qed.
+Defined.
 
 Program Definition inc (k:nat) :
   forall (st_pre : ST_Pre) (A:Set) (st_post : ST_Post A) (c_post : C_Post A),
     CS st_pre A st_post
-    (fun a an =>
+    (fun st a an st' =>
       forall am,
         an + k = am ->
-        c_post a am) ->
+        c_post st a am st') ->
     CS st_pre A st_post c_post.
 Proof.
   intros. rename H into am.
@@ -114,5 +113,62 @@ Proof.
   exists (an + k).
   eapply c_post_stA.
   auto.
-Qed.
+Defined.
+
+End monad.
     
+(* xxx example inline for testing *)
+Section dumb_list.
+
+Definition ST := list nat.
+
+Program Fixpoint list_insert x (l:ST) : ST :=
+  match l with
+    | nil =>
+      cons x nil
+    | cons y l =>
+      cons y (list_insert x l)
+  end.
+
+Program Definition insert (x:nat) :
+  @CS ST
+  (fun st => True)
+  ()
+  (fun st _ st' => st' = list_insert x st)
+  (fun st _ n st' => n = length st)
+  :=
+  @bind ST ST ()
+  (fun st => True)
+  (fun st0v st0 => st0v = st0)
+  (fun st0 st1 st2 => st0 = st1 /\ st1 = st2)
+  (fun st0v st0 _ st2 => st2 = list_insert x st0)
+  (fun st0 st0v getn st1 => getn = 0)
+  (fun st0 _ putn st2 => putn = length st0)
+  (@get ST)
+  (fun l =>
+    (@put ST (list_insert x l))).
+
+Next Obligation.
+  unfold top. auto.
+Defined.
+
+Next Obligation.
+  rename x0 into st0.
+  split. auto.
+
+  (* XXX *)
+  exists (length st
+  
+  eauto.
+  
+  destruct (`
+       (put ST (list_insert x st0)
+          (exist (fun st : ST => top ST st) st0
+             (insert_obligation_1 x st0
+                (exist (fun st : ST => st0 = st) st0 eq_refl))))) as [u st1].
+  
+  split.
+ simpl.
+
+End dumb_list.
+
